more

FSets_Bags.thy
@@ -35,20 +35,20 @@ where
 by (auto simp: BIns)
 
 (* Membership of an item in a finite set *)
-nonfreeiter mem :: "'a fset \<Rightarrow> 'a \<Rightarrow> bool"
+nonfreeiter mem :: "'a \<Rightarrow> 'a fset \<Rightarrow> bool"
 where
-  "mem Emp = (\<lambda> a. False)"
-| "mem (Ins b B) = (\<lambda> a. a = b \<or> mem B a)"
-by (auto intro!: ext)
+  "mem a Emp = False"
+| "mem a (Ins b B) = (a = b \<or> mem a B)"
+by auto
 
-lemma mem_Ins[simp]: "mem A a \<Longrightarrow> Ins a A = A"
+lemma mem_Ins[simp]: "mem a A \<Longrightarrow> Ins a A = A"
 by (induction arbitrary: a rule: fset_induct) (auto simp: Ins2)
 
 (* Multiplicity of an item in bag *)
-nonfreeiter mult :: "'a bag \<Rightarrow> 'a \<Rightarrow> nat"
+nonfreeiter mult :: "'a \<Rightarrow> 'a bag \<Rightarrow> nat"
 where
-  "mult BEmp = (\<lambda> a. 0)"
-| "mult (BIns b B) = (\<lambda> a. if a = b then Suc (mult B a) else mult B a)"
+  "mult a BEmp = 0"
+| "mult a (BIns b B) = (if a = b then Suc (mult a B) else mult a B)"
 by (auto simp: BIns)
 
 (* Flattening operator from bags to finite sets *)
@@ -56,26 +56,26 @@ nonfreeiter flat :: "'a bag \<Rightarrow> 'a fset"
 where
   "flat BEmp = Emp"
 | "flat (BIns a B) = Ins a (flat B)"
-by (auto simp: Ins1 Ins2)
+by (auto simp: Ins2)
 
-lemma mem_flat_mult[simp]: "mem (flat A) a \<longleftrightarrow> mult A a \<noteq> 0"
+lemma mem_flat_mult[simp]: "mem a (flat A) \<longleftrightarrow> mult a A \<noteq> 0"
 by (induction rule: bag_induct) auto
 
 (* Embedding of finite sets into bags *)
 nonfreeiter embed :: "'a fset \<Rightarrow> 'a bag"
 where
   "embed Emp = BEmp"
-| "embed (Ins a A) = (if mult (embed A) a = 0 then BIns a (embed A) else embed A)"
+| "embed (Ins a A) = (if mult a (embed A) = 0 then BIns a (embed A) else embed A)"
 by (auto simp: BIns)
 
-lemma mult_embed_mem[simp]: "mult (embed A) a \<noteq> 0 \<longleftrightarrow> mem A a"
+lemma mult_embed_mem[simp]: "mult a (embed A) \<noteq> 0 \<longleftrightarrow> mem a A"
 by (induction rule: fset_induct) auto
 
 (* Cardinal of finite sets: *)
 nonfreeiter card1 :: "'a fset \<Rightarrow> 'a fset * nat"
 where
   "card1 Emp = (Emp, 0)"
-| "card1 (Ins a A) = (case card1 A of (A,n) \<Rightarrow> (Ins a A, if mem A a then n else Suc n))"
+| "card1 (Ins a A) = (case card1 A of (A,n) \<Rightarrow> (Ins a A, if mem a A then n else Suc n))"
 by (auto simp: Ins2)
 
 lemma card1: "card1 A = (A',n) \<Longrightarrow> A = A'"
@@ -85,40 +85,39 @@ definition card :: "'a fset \<Rightarrow> nat" where "card \<equiv> snd o card1"
 
 lemma card_simps[simp]:
   "card Emp = 0"
-  "card (Ins a A) = (if mem A a then card A else Suc (card A))"
+  "card (Ins a A) = (if mem a A then card A else Suc (card A))"
 unfolding card_def using card1 by (auto split: prod.splits)
 
 (* Sum of a numeric function over a finite set: *)
-nonfreeiter sum1 :: "'a fset \<Rightarrow> 'a fset \<times> (('a \<Rightarrow> nat) \<Rightarrow> nat)"
+nonfreeiter sum1 :: "('a \<Rightarrow> nat) \<Rightarrow> 'a fset \<Rightarrow> 'a fset \<times> nat"
 where
-  "sum1 Emp = (Emp, (\<lambda> f. 0))"
-| "sum1 (Ins a A) = (case sum1 A of (A,S) \<Rightarrow> (Ins a A, if mem A a then S else (\<lambda> f. S f  + f a)))"
+  "sum1 f Emp = (Emp, 0)"
+| "sum1 f (Ins a A) = (case sum1 f A of (A,n) \<Rightarrow> (Ins a A, if mem a A then n else n + f a))"
 by (auto simp: Ins2)
 
-lemma sum1: "sum1 A = (A',n) \<Longrightarrow> A = A'"
+lemma sum1: "sum1 f A = (A',n) \<Longrightarrow> A = A'"
 by (induct arbitrary: A' n rule: fset_induct) (auto split: prod.splits)
 
-definition sum :: "'a fset \<Rightarrow> ('a \<Rightarrow> nat) \<Rightarrow> nat" where "sum \<equiv> snd o sum1"
+definition sum :: " ('a \<Rightarrow> nat) \<Rightarrow> 'a fset \<Rightarrow> nat" where "sum f \<equiv> snd o sum1 f"
 
 lemma sum_simps[simp]:
-  "sum Emp f = 0"
-  "sum (Ins a A) f = (if mem A a then sum A f else sum A f + f a)"
+  "sum f Emp = 0"
+  "sum f (Ins a A) = (if mem a A then sum f A else sum f A + f a)"
 unfolding sum_def using sum1 by (auto split: prod.splits)
 
 (* Sum of a numeric function over a bag: *)
-nonfreeiter bsum :: "'a bag \<Rightarrow> ('a \<Rightarrow> nat) \<Rightarrow> nat"
+nonfreeiter bsum' :: "('a \<Rightarrow> nat) \<Rightarrow> 'a bag \<Rightarrow> nat"
 where
-  "bsum BEmp = (\<lambda> f. 0)"
-| "bsum (BIns a B) = (\<lambda> f. bsum B f + f a)"
+  "bsum' f BEmp = 0"
+| "bsum' f (BIns a B) = bsum' f B + f a"
 by auto
 
 (* More generally: Sum of a commutative-monoid-valed function over a bag: *)
-nonfreeiter bsum_gen :: "'a bag \<Rightarrow> ('a \<Rightarrow> ('b::comm_monoid_add)) \<Rightarrow> 'b"
+nonfreeiter bsum :: "('a \<Rightarrow> 'b::comm_monoid_add) \<Rightarrow> 'a bag \<Rightarrow> 'b"
 where
-  "bsum_gen BEmp = (\<lambda> f. 0)"
-| "bsum_gen (BIns a B) = (\<lambda> f. bsum_gen B f + f a)"
+  "bsum f BEmp = 0"
+| "bsum f (BIns a B) = bsum f B + f a"
 by (auto simp: algebra_simps)
-
 
 (* Embedding of finite sets as sets: *)
 nonfreeiter asSet :: "'a fset \<Rightarrow> 'a set"
@@ -127,10 +126,10 @@ where
 | "asSet (Ins a A) = insert a (asSet A)"
 by auto
 
-lemma in_asSet[simp]: "a \<in> asSet F \<longleftrightarrow> mem F a"
+lemma in_asSet[simp]: "a \<in> asSet F \<longleftrightarrow> mem a F"
 by (induction F) auto
 
-lemma mem_ex_Ins: "mem F a \<Longrightarrow> \<exists> F'. \<not> mem F' a \<and> F = Ins a F'"
+lemma mem_ex_Ins: "mem a F \<Longrightarrow> \<exists> F'. \<not> mem a F' \<and> F = Ins a F'"
 by (induction F) (metis Ins2 mem.simps mem_Ins)+
 
 lemma finite_asSet[simp, intro]: "finite (asSet A)"
@@ -146,10 +145,10 @@ lemma asSet_inj[simp]: "asSet F1 = asSet F2 \<longleftrightarrow> F1 = F2"
 proof(safe, induction F1 arbitrary: F2)
   fix a F1 F2 assume IH: "\<And>F2. asSet F1 = asSet F2 \<Longrightarrow> F1 = F2"
   and e: "asSet (Ins a F1) = asSet F2"
-  hence "mem F2 a" by auto
-  then obtain F2' where F2': "\<not> mem F2' a" and F2: "F2 = Ins a F2'" using mem_ex_Ins[of F2 a] by blast
+  hence "mem a F2" by auto
+  then obtain F2' where F2': "\<not> mem a F2'" and F2: "F2 = Ins a F2'" using mem_ex_Ins[of a F2] by blast
   show "Ins a F1 = F2"
-  proof(cases "mem F1 a")
+  proof(cases "mem a F1")
     case False
     hence "asSet F1 = asSet F2'" using e F2' unfolding F2 by auto
     thus ?thesis unfolding F2 using IH by auto
@@ -181,7 +180,7 @@ assumes "\<And>a b. I a (I a b) = I a b"
 and "\<And> a1 a2 b. I a1 (I a2 b) = I a2 (I a1 b)"
 shows "fold_fset E I {} = E"
 unfolding fold_fset_def comp_def asSet.simps(1)[symmetric] asFset_asSet
-apply(rule iter_op_clauses942546(1)) using assms by auto
+apply(rule iter_op_clauses684605(1)) using assms by auto
 
 lemma fold_fset_insert:
 assumes A: "finite A"
@@ -189,7 +188,7 @@ and "\<And>a b. I a (I a b) = I a b"
 and "\<And> a1 a2 b. I a1 (I a2 b) = I a2 (I a1 b)"
 shows "fold_fset E I (insert a A) = I a (fold_fset E I A)"
 unfolding fold_fset_def comp_def asSet.simps(2)[symmetric] asFset_asSet asFset_insert[OF A]
-apply(rule iter_op_clauses942546(2)) using assms by auto
+apply(rule iter_op_clauses684605(2)) using assms by auto
 
 (* ACIU view: *)
 definition "Singl a \<equiv> Ins a Emp"
