Reg_Exp.thy
@@ -1,0 +1,27 @@
+theory Reg_Exp
+imports NonFree
+uses "input.ML"
+begin
+
+nonfreedata 'a exp = Eps | Let 'a | Plus "'a exp" "'a exp" |
+                     Times "'a exp" "'a exp" | Star "'a exp"
+where
+   Plus_Assoc: "Plus (Plus e1 e2) e3 = Plus e1 (Plus e2 e3)"
+ | Plus_Comm: "Plus e1 e2 = Plus e2 e1"
+ | Plus_Idem: "Plus e e = e"
+ | Plus_Eps: "Plus Eps e = e"
+ | Times_Eps: "Times Eps e = Eps"
+ | Distr: "Times e1 (Plus e2 e3) = Plus (Times e1 e2) (Times e1 e3)"
+
+nonfreeiter lang :: "'a exp \<Rightarrow> 'a list set"
+where
+  "lang Eps = {}"
+| "lang (Let a) = {[a]}"
+| "lang (Plus e1 e2) = lang e1 \<union> lang e2"
+| "lang (Times e1 e2) = { w1 @ w2 | w1 w2. w1 \<in> lang e1 \<and> w2 \<in> lang e2}"
+| "lang (Star e) = { List.concat ws | ws. set ws \<subseteq> lang e}"
+by auto
+
+
+
+end
